Eternity2/SATSolve.lean
@@ -1,0 +1,32 @@
+import Eternity2.EncCNF
+
+namespace SATSolve
+
+open Std EncCNF
+
+def runCadical (cnfFile : String) : IO (Option (HashMap Var Bool)) := do
+  -- Run cadical on cnfFile
+  let out := (← IO.Process.output {
+    stdin := .piped
+    stdout := .piped
+    stderr := .piped
+    cmd := "cadical"
+    args := #[cnfFile, "--sat", "-f", "-q"]
+  }).stdout
+  let lines := out.splitOn "\n" |>.filter (not <| String.startsWith "c" ·)
+  match lines with
+  | "s SATISFIABLE" :: satis =>
+    return some (
+      satis
+      |>.filter (not <| ·.isEmpty)
+      |>.map (·.drop 2 |>.splitOn " ")
+      |>.join
+      |>.map (·.toInt!)
+      |>.filter (· ≠ 0)
+      |>.foldl (fun acc i =>
+          acc.insert (Int.natAbs i - 1) (i > 0)
+        ) (HashMap.empty)
+    )
+  | "s UNSATISFIABLE" :: _ => return none
+  | out =>
+    panic! s!"failed to parse output ({out.length} lines):\n{out.take 3}\n..."
