Eternity2/TileSet.lean
@@ -4,6 +4,14 @@ namespace Eternity2
 
 def TileSet := List Tile
 
+def TileSet.toFile (filename : String) (ts : TileSet) : IO Unit := do
+  let size := Nat. ts.length
+  let contents :=
+    s!"p tile 16 16\n" ++
+    String.intercalate "\n" (ts.map (fun ⟨u,d,l,r,_⟩ => s!"{u} {r} {d} {l}"))
+  IO.FS.withFile filename .write (fun handle =>
+    handle.putStr contents)
+
 def TileSet.fromFile (filename : String) : IO TileSet := do
   let contents ← IO.FS.withFile filename .read (fun handle =>
     handle.readToEnd
@@ -12,7 +20,8 @@ def TileSet.fromFile (filename : String) : IO TileSet := do
     |>.filter (!·.startsWith "c")
     |>.dropWhile (fun s => !s.startsWith "p")
     |>.drop 1
+    |>.filter (!·.all Char.isWhitespace)
     |>.map (fun s =>
       match s.splitOn " " |>.map String.toNat? with
-      | [some a, some b, some c, some d] => ⟨a,b,c,d,none⟩
+      | [some a, some b, some c, some d] => ⟨a,c,d,b,none⟩
       | _ => panic! s!"Bad input line {s}")
